wip

crypto/bignum/Hacl.Bignum.Fdifference.fst
@@ -6,31 +6,11 @@ open FStar.Buffer
 open Hacl.Bignum.Parameters
 open Hacl.Bignum.Bigint
 open Hacl.Bignum.Limb
-
+open Hacl.Bignum.Fdifference.Spec
 
 module U32 = FStar.UInt32
 
-type seqelem = s:Seq.seq limb{Seq.length s = len}
-
-
-let gte_limbs (a:seqelem) (b:seqelem) (l:nat{l <= len}) : GTot Type0 =
-  (forall (i:nat). {:pattern (Seq.index a i) \/ (Seq.index b i)} i < l ==> v (Seq.index b i) >= v (Seq.index a i))
-
-
-val fdifference_spec:
-  a:seqelem -> b:seqelem ->
-  ctr:nat{ctr <= len /\ gte_limbs a b ctr} ->
-  Tot seqelem (decreases ctr)
-let rec fdifference_spec a b ctr =
-  if ctr = 0 then a
-  else (
-    let i = ctr - 1 in
-    let ai = Seq.index a i in
-    let bi = Seq.index b i in
-    let a' = Seq.upd a i (bi -^ ai) in
-    fdifference_spec a' b i
-  )
-
+#set-options "--initial_fuel 1 --max_fuel 1 --z3timeout 20"
 
 let gte_limbs_c h (a:felem) h' (b:felem) (l:nat{l <= len}) : GTot Type0 =
   live h a /\ live h' b /\ gte_limbs (as_seq h a) (as_seq h' b) l
@@ -52,13 +32,3 @@ let rec fdifference_ a b i =
     a.(i) <- bi -^ ai;
     fdifference_ a b i
   )
-
-
-(* val fdifference: *)
-(*   a:felem -> *)
-(*   b:felem -> *)
-(*   Stack unit *)
-(*     (requires (fun h -> gte_limbs_c h b h a len)) *)
-(*     (ensures  (fun h0 _ h1 -> is_subtraction h1 a h0 b 0)) *)
-(* let fdifference a b = *)
-(*   fdifference_ a b clen *)
