crypto/bignum/Hacl.Bignum.Fproduct.fst
@@ -8,46 +8,11 @@ open Hacl.Bignum.Parameters
 open Hacl.Bignum.Bigint
 open Hacl.Bignum.Limb
 open Hacl.Bignum.Modulo
+open Hacl.Bignum.Fproduct.Spec
 
 module U32 = FStar.UInt32
 
-
-type seqelem = s:Seq.seq limb{Seq.length s = len}
-type seqelem_wide = s:Seq.seq wide{Seq.length s = len}
-
-
-let copy_from_wide_pre (s:seqelem_wide) : GTot Type0 =
-  (forall (i:nat). {:pattern w (Seq.index s i)} i < len ==> w (Seq.index s i) < pow2 n)
-
-
-#set-options "--z3timeout 20"
-
-val copy_from_wide_spec_: s:seqelem_wide{copy_from_wide_pre s} ->
-  i:nat{i <= len} ->
-  tmp:seqelem{(forall (j:nat). (j >= i /\ j < len) ==> v (Seq.index tmp j) = w (Seq.index s j))} ->
-  Tot (s':seqelem{(forall (j:nat). j < len ==> v (Seq.index s' j) = w (Seq.index s j))})
-let rec copy_from_wide_spec_ s i tmp =
-  if i = 0 then tmp
-  else (
-    let i = i - 1 in
-    let si = Seq.index s i in
-    let tmpi = wide_to_limb si in
-    Math.Lemmas.modulo_lemma (w si) (pow2 n);
-    let tmp' = Seq.upd tmp i tmpi in
-    copy_from_wide_spec_ s i tmp'
-  )
-
-
-#set-options "--z3timeout 5"
-
-val copy_from_wide_spec: s:seqelem_wide{copy_from_wide_pre s} ->
-  Tot (s':seqelem{(forall (j:nat). j < len ==> v (Seq.index s' j) = w (Seq.index s j))})
-let rec copy_from_wide_spec s =
-  let tmp = Seq.create len limb_zero in
-  copy_from_wide_spec_ s len tmp
-
-
-#set-options "--z3timeout 50"
+#set-options "--z3timeout 50 --initial_fuel 1 --max_fuel 1"
 
 val copy_from_wide_:
   output:felem ->
@@ -73,14 +38,6 @@ let rec copy_from_wide_ output input ctr =
     copy_from_wide_ output input i
   )
 
-
-#set-options "--z3timeout 5"
-
-val shift_spec: seqelem -> Tot seqelem
-let shift_spec s =
-  let sfirst = Seq.slice s 0 (len - 1) in
-  let slast = Seq.slice s (len-1) len in
-  Seq.append slast sfirst
 
 #set-options "--z3timeout 50"
 
@@ -119,32 +76,7 @@ let rec shift output =
   let h = ST.get() in
   Seq.lemma_eq_intro (as_seq h output) (shift_spec (as_seq h0 output))
 
-#set-options "--z3timeout 20 --initial_fuel 1 --max_fuel 1"
-
-open FStar.Mul
-
-let sum_scalar_multiplication_pre_ (sw:seqelem_wide) (s:seqelem) (scalar:limb) (i:nat{i <= len}) : GTot Type0 =
-  (forall (j:nat). j < i ==> w (Seq.index sw j) + (v (Seq.index s j) * v scalar) < pow2 wide_n)
-
-
-val sum_scalar_multiplication_spec:
-  sw:seqelem_wide ->
-  s:seqelem ->
-  scalar:limb ->
-  i:nat{i <= len /\ sum_scalar_multiplication_pre_ sw s scalar i} ->
-  Tot seqelem_wide
-  (decreases i)
-let rec sum_scalar_multiplication_spec sw s scalar i =
-  if i = 0 then sw
-  else (
-    let j = i - 1 in
-    let swi = Seq.index sw j in
-    let si = Seq.index s j in
-    let open Hacl.Bignum.Wide in
-    let swi' = swi +^ (mul_wide si scalar) in
-    let sw' = Seq.upd sw j swi' in
-    sum_scalar_multiplication_spec sw' s scalar j
-  )
+#set-options "--z3timeout 20"
 
 
 #set-options "--z3timeout 20 --initial_fuel 1 --max_fuel 1"
@@ -171,13 +103,6 @@ let rec sum_scalar_multiplication_ output input s ctr =
   )
 
 
-let shift_reduce_pre (s:seqelem) : GTot Type0 = reduce_pre (shift_spec s)
-
-val shift_reduce_spec: s:seqelem{shift_reduce_pre s} -> Tot (s':seqelem)
-let shift_reduce_spec s =
-  reduce_spec (shift_spec s)
-
-
 val shift_reduce: output:felem -> Stack unit
   (requires (fun h -> live h output /\ shift_reduce_pre (as_seq h output)))
   (ensures (fun h0 _ h1 -> live h0 output /\ live h1 output /\ modifies_1 output h0 h1
@@ -186,35 +111,6 @@ val shift_reduce: output:felem -> Stack unit
 let shift_reduce output =
   shift output;
   reduce output
-
-
-
-let rec mul_shift_reduce_pre (output:seqelem_wide) (input:seqelem) (input2:seqelem) (ctr:nat{ctr <= len}) : GTot Type0 (decreases ctr) =
-  if ctr > 0 then (
-    sum_scalar_multiplication_pre_ output input (Seq.index input2 (len-ctr)) len
-    /\ (let output' = sum_scalar_multiplication_spec output input (Seq.index input2 (len-ctr)) len in
-       (ctr > 1 ==> shift_reduce_pre input) /\
-         (let input'  = if ctr > 1 then shift_reduce_spec input else input in
-          mul_shift_reduce_pre output' input' input2 (ctr-1))))
-          else true
-
-
-val mul_shift_reduce_spec:
-  output:seqelem_wide ->
-  input:seqelem -> input2:seqelem ->
-  ctr:nat{ctr <= len /\ mul_shift_reduce_pre output input input2 ctr} ->
-  Tot seqelem_wide
-  (decreases ctr)
-let rec mul_shift_reduce_spec output input input2 ctr =
-  if ctr = 0 then output
-  else (
-    let i = ctr - 1 in
-    let j = len - i - 1 in
-    let input2j = Seq.index input2 j in
-    let output' = sum_scalar_multiplication_spec output input input2j len in
-    let input'  = if ctr > 1 then shift_reduce_spec input else input in
-    mul_shift_reduce_spec output' input' input2 i
-  )
 
 #set-options "--z3timeout 50 --initial_fuel 1 --max_fuel 1"
 
@@ -244,33 +140,10 @@ let rec mul_shift_reduce_ output input input2 ctr =
   )
 
 
-#set-options "--z3timeout 10 --initial_fuel 1 --max_fuel 1"
-
-let carry_wide_pre (s:seqelem_wide) (i:nat{i < len}) : GTot Type0 =
-  w (Seq.index s i) < pow2 wide_n
-  /\ (forall (j:nat). (j > i /\ j < len) ==> w (Seq.index s j) < pow2 (wide_n - 1))
-
-
-#set-options "--lax"
-
-val carry_wide_spec: s:seqelem_wide -> i:nat{i < len} -> Tot (s':seqelem_wide)
-let rec carry_wide_spec s i =
-  if i = len - 1 then s
-  else (
-    let si = Seq.index s i in
-    let sip1 = Seq.index s (i+1) in
-    let r0 = wide_to_limb si &^ ((limb_one <<^ climb_size) -^ limb_one) in
-    let open Hacl.Bignum.Wide in
-    let c = wide_to_limb (si >>^ climb_size) in
-    let s' = Seq.upd s i (limb_to_wide r0) in
-    let s'' = Seq.upd s (i+1) (sip1 +^ limb_to_wide c) in
-    carry_wide_spec s'' (i+1)
-  )
-
 
 val carry_wide_:
   t:felem_wide ->
-  ctr:U32.t ->
+  ctr:U32.t{U32.v ctr < len} ->
   Stack unit
     (requires (fun h -> live h t /\ carry_wide_pre (as_seq h t) (U32.v ctr)))
     (ensures (fun h0 _ h1 -> live h0 t /\ live h1 t /\ modifies_1 t h0 h1
@@ -281,38 +154,120 @@ let rec carry_wide_ t ctr =
   else (
     let tctr = t.(ctr) in
     let tctrp1 = t.(U32 (ctr+^1ul)) in
+    assert_norm(pow2 0 = 1);
+    Math.Lemmas.pow2_lt_compat limb_size 0;
+    Math.Lemmas.pow2_lt_compat limb_n limb_size;
+    Math.Lemmas.modulo_lemma (pow2 limb_size) (pow2 limb_n);
     let r0 = wide_to_limb (tctr) &^ ((limb_one <<^ climb_size) -^ limb_one) in
+    UInt.logand_mask #limb_n (v (wide_to_limb tctr)) limb_size;
+    Math.Lemmas.pow2_plus (limb_n - limb_size) (limb_size);
+    Math.Lemmas.modulo_modulo_lemma (w tctr) (pow2 limb_size) (pow2 (limb_n - limb_size));
+    assert(v r0 = w tctr % pow2 limb_size);
+    assert(v r0 < pow2 limb_size);
     let open Hacl.Bignum.Wide in
-    let c  = wide_to_limb (tctr >>^ climb_size) in
+    let c  = tctr >>^ climb_size in
+    Math.Lemmas.pow2_lt_compat (wide_n - 1) (limb_n);
+    Math.Lemmas.pow2_double_sum (wide_n - 1);
+    Math.Lemmas.lemma_div_lt (w tctr) (wide_n) (limb_size);
+    Math.Lemmas.pow2_le_compat (wide_n - 1) (wide_n - limb_size);
     t.(ctr) <- limb_to_wide r0;
-    t.(U32 (ctr +^ 1ul)) <- tctrp1 +^ limb_to_wide c;
+    t.(U32 (ctr +^ 1ul)) <- tctrp1 +^ c;
     carry_wide_ t (U32 (ctr +^ 1ul))
   )
 
-  
-val fmul:
+
+#set-options "--z3timeout 5"
+
+#set-options "--z3timeout 20"
+
+val carry_0_to_1:
+  output:felem ->
+  Stack unit
+    (requires (fun h -> live h output /\ carry_0_to_1_pre (as_seq h output)))
+    (ensures (fun h0 _ h1 -> live h0 output /\ live h1 output /\ modifies_1 output h0 h1
+      /\ carry_0_to_1_pre (as_seq h0 output)
+      /\ as_seq h1 output == carry_0_to_1_spec (as_seq h0 output)))
+let carry_0_to_1 output =
+  assume (length output > 1);
+  let i0 = output.(0ul) in
+  let i1 = output.(1ul) in
+  assert_norm(pow2 0 = 1);
+  Math.Lemmas.pow2_lt_compat limb_size 0;
+  Math.Lemmas.pow2_lt_compat limb_n limb_size;
+  Math.Lemmas.modulo_lemma (pow2 limb_size) (pow2 limb_n);
+  UInt.logand_mask #limb_n (v i0) limb_size;
+  Math.Lemmas.pow2_plus (limb_n - limb_size) (limb_size);
+  Math.Lemmas.modulo_modulo_lemma (v i0) (pow2 limb_size) (pow2 (limb_n - limb_size));
+  Math.Lemmas.pow2_double_sum (limb_n - 1);
+  Math.Lemmas.pow2_le_compat (limb_n - 1) limb_size;
+  Math.Lemmas.lemma_div_lt (v i0) (limb_n) (limb_size);
+  Math.Lemmas.pow2_le_compat (limb_n - 1) (limb_n - limb_size);
+  let i0' = i0 &^ ((limb_one <<^ climb_size) -^ limb_one) in
+  cut (v i1 < pow2 (limb_size));
+  let i1'   = i1 +^ (i0 >>^ climb_size) in
+  output.(0ul) <- i0';
+  output.(1ul) <- i1'
+
+#set-options "--z3timeout 40"
+
+
+val fmul_:
   output:felem ->
   input:felem{disjoint output input} ->
   input2:felem{disjoint output input2 /\ disjoint input input2} ->
   Stack unit
-    (requires (fun h -> live h output /\ live h input /\ live h input2))
-    (ensures (fun h0 _ h1 -> modifies_2 output input h0 h1 /\ live h1 output /\ live h1 input))
-let fmul output input input2 =
+    (requires (fun h -> live h output /\ live h input /\ live h input2
+      /\ fmul_pre (as_seq h input) (as_seq h input2)))
+    (ensures (fun h0 _ h1 -> live h0 output /\ live h0 output /\ live h0 input /\ live h0 input2 
+      /\ modifies_2 output input h0 h1 /\ live h1 output /\ live h1 input
+      /\ fmul_pre (as_seq h0 input) (as_seq h0 input2)
+      /\ as_seq h1 output == fmul_spec (as_seq h0 input) (as_seq h0 input2)
+      ))
+let fmul_ output input input2 =
+  let h0 = ST.get() in
+  lemma_mul_to_red (as_seq h0 input) (as_seq h0 input2);
   push_frame();
-  let tmp = create limb_zero clen in
+  let h1 = ST.get() in
   let t   = create wide_zero clen in
-  blit input 0ul tmp 0ul clen;
-  mul_shift_reduce_ t tmp input2 clen;
+  let h2 = ST.get() in
+  mul_shift_reduce_ t input input2 clen;
   carry_wide_ t 0ul;
   reduce_wide t;
   copy_from_wide_ output t clen;
-  let output0 = output.(0ul) in
-  let output1 = output.(1ul) in
-  let c = output0 >>^ climb_size in
-  output.(0ul) <- output0 &^ ((limb_one <<^ climb_size) -^ limb_one);
-  output.(1ul) <- output1 +^ c;
+  carry_0_to_1 output;
+  let h3 = ST.get() in
+  assume (modifies_2 output input h1 h3);
   pop_frame()
 
+
+val fmul:
+  output:felem ->
+  input:felem{disjoint output input} ->
+  input2:felem{disjoint output input2} ->
+  Stack unit
+    (requires (fun h -> live h output /\ live h input /\ live h input2
+      /\ fmul_pre (as_seq h input) (as_seq h input2)))
+    (ensures (fun h0 _ h1 -> live h0 output /\ live h0 output /\ live h0 input /\ live h0 input2 
+      /\ modifies_1 output h0 h1 /\ live h1 output
+      /\ fmul_pre (as_seq h0 input) (as_seq h0 input2)
+      /\ as_seq h1 output == fmul_spec (as_seq h0 input) (as_seq h0 input2)
+      ))
+let fmul output input input2 =
+  let h0 = ST.get() in
+  lemma_mul_to_red (as_seq h0 input) (as_seq h0 input2);
+  push_frame();
+  let h1 = ST.get() in
+  let tmp = create limb_zero clen in
+  blit input 0ul tmp 0ul clen;
+  let h2 = ST.get() in
+  lemma_whole_slice (as_seq h2 input);
+  lemma_whole_slice (as_seq h2 tmp);
+  fmul_ output tmp input2;
+  let h3 = ST.get() in
+  pop_frame()
+
+
+#set-options "--lax"
 
 val fsquare_times_:
   input:felem ->
