crypto/bignum/Hacl.Bignum.Fscalar.fst
@@ -6,25 +6,11 @@ open FStar.Buffer
 open Hacl.Bignum.Parameters
 open Hacl.Bignum.Bigint
 open Hacl.Bignum.Limb
-
+open Hacl.Bignum.Fscalar.Spec
 
 module U32 = FStar.UInt32
 
-type seqelem = s:Seq.seq limb{Seq.length s = len}
-type seqelem_wide = s:Seq.seq wide{Seq.length s = len}
-
-
-val fscalar_spec: output:seqelem_wide -> input:seqelem -> s:limb -> ctr:nat{ctr <= len} -> Tot seqelem_wide (decreases ctr)
-let rec fscalar_spec output input s ctr =
-  if ctr = 0 then output
-  else (
-    let i = ctr - 1 in
-    let inputi = Seq.index input i in
-    let open Hacl.Bignum.Wide in
-    let output' = Seq.upd output i (inputi *^ s) in
-    fscalar_spec output' input s i
-  )
-
+#set-options "--initial_fuel 1 --max_fuel 1 --z3timeout 20"
 
 val fscalar_:
   output:felem_wide ->
