crypto/bignum/Hacl.Bignum.Fsum.fst
@@ -7,33 +7,13 @@ open Hacl.Bignum.Parameters
 open Hacl.Bignum.Bigint
 open Hacl.Bignum.Limb
 open Hacl.Bignum.Predicates
-
+open Hacl.Bignum.Fsum.Spec
 
 module U32 = FStar.UInt32
 
-
-type seqelem = s:Seq.seq limb{Seq.length s = len}
-
-
-let red (s:seqelem) (l:nat{l <= len}) = (forall (i:nat). (i < l) ==> v (Seq.index s i) < pow2 (n - 1))
-
-
-val fsum_spec: s:seqelem -> s':seqelem -> ctr:nat{ctr <= len /\ red s ctr /\ red s' ctr} -> Tot seqelem
-  (decreases ctr)
-let rec fsum_spec a b ctr =
-  if ctr = 0 then a
-  else (
-    let i = ctr - 1 in
-    let ai = Seq.index a i in
-    let bi = Seq.index b i in
-    Math.Lemmas.pow2_double_sum (n-1);
-    let a' = Seq.upd a i (ai +^ bi) in
-    fsum_spec a' b i
-  )
-
+#set-options "--initial_fuel 1 --max_fuel 1 --z3timeout 20"
 
 let red_c h (f:felem) ctr = live h f /\ red (as_seq h f) ctr
-
 
 val fsum_:
   a:felem ->
