crypto/bignum/Hacl.Bignum.Parameters.fsti
@@ -3,26 +3,28 @@ module Hacl.Bignum.Parameters
 open FStar.Mul
 open FStar.HyperStack
 open FStar.Buffer
+open Hacl.Bignum.Constants
 
 (** The values of the prime for modular arithmetic **)
-val prime: pos
+inline_for_extraction let prime = prime
 
 (** Size of a word on the platform (32 or 64bits) **)
-val word_size: ws:pos
+inline_for_extraction let word_size = word_size
 
 (** Concrete platform word with side-channel protection **)
 inline_for_extraction val limb: Type0
 inline_for_extraction val wide: Type0
 inline_for_extraction let ctr  = FStar.UInt32.t
 
-
 (** Number of limbs of a bigint **)
-val len: pos
+inline_for_extraction let len = len
 inline_for_extraction val clen: l:FStar.UInt32.t{FStar.UInt32.v l = len}
 
 type felem = b:buffer limb{length b = len}
 type felem_wide = b:buffer wide{length b = len}
 
+type seqelem = s:Seq.seq limb{Seq.length s = len}
+type seqelem_wide = s:Seq.seq wide{Seq.length s = len}
 
 (** Associates a weight in bits to each limb of the bigint *)
 val limb_size: s:pos{s < word_size}
@@ -53,10 +55,10 @@ inline_for_extraction val limb_mul: a:limb -> b:limb{UInt.size (v a * v b) limb_
 inline_for_extraction val limb_mul_mod: a:limb -> b:limb -> Tot (c:limb{(v a * v b) % pow2 limb_n = v c})
 
 (* Bitwise operators *)
-inline_for_extraction val limb_logand: limb -> limb -> Tot limb
-inline_for_extraction val limb_logxor: limb -> limb -> Tot limb
-inline_for_extraction val limb_logor: limb -> limb -> Tot limb
-inline_for_extraction val limb_lognot: limb -> Tot limb
+inline_for_extraction val limb_logand: a:limb -> b:limb -> Tot (c:limb{v c = UInt.logand (v a) (v b)})
+inline_for_extraction val limb_logxor: a:limb -> b:limb -> Tot (c:limb{v c = UInt.logxor (v a) (v b)})
+inline_for_extraction val limb_logor: a:limb -> b:limb -> Tot (c:limb{v c = UInt.logor (v a) (v b)})
+inline_for_extraction val limb_lognot: a:limb -> Tot (b:limb{v b = UInt.lognot (v a)})
 
 (* Shift operators *)
 inline_for_extraction val limb_shift_right: a:limb -> s:FStar.UInt32.t -> Tot (c:limb{FStar.UInt32.v s < limb_n ==> v c = (v a / (pow2 (FStar.UInt32.v s)))})
@@ -92,10 +94,10 @@ inline_for_extraction val wide_add_mod: a:wide -> b:wide -> Tot (c:wide{(w a + w
 inline_for_extraction val wide_sub: a:wide -> b:wide{UInt.size (w a - w b) wide_n} -> Tot (c:wide{w a - w b = w c})
 inline_for_extraction val wide_sub_mod: a:wide -> b:wide -> Tot (c:wide{(w a - w b) % pow2 wide_n = w c})
 (* Bitwise operators *)
-inline_for_extraction val wide_logand: wide -> wide -> Tot wide
-inline_for_extraction val wide_logxor: wide -> wide -> Tot wide
-inline_for_extraction val wide_logor: wide -> wide -> Tot wide
-inline_for_extraction val wide_lognot: wide -> Tot wide
+inline_for_extraction val wide_logand: a:wide -> b:wide -> Tot (c:wide{w c = UInt.logand (w a) (w b)})
+inline_for_extraction val wide_logxor: a:wide -> b:wide -> Tot (c:wide{w c = UInt.logxor (w a) (w b)})
+inline_for_extraction val wide_logor: a:wide -> b:wide -> Tot (c:wide{w c = UInt.logor (w a) (w b)})
+inline_for_extraction val wide_lognot: a:wide -> Tot (b:wide{w b = UInt.lognot (w a)})
 
 (* Shift operators *)
 inline_for_extraction val wide_shift_right: a:wide -> s:FStar.UInt32.t -> Tot (c:wide{FStar.UInt32.v s < wide_n ==> w c = (w a / (pow2 (FStar.UInt32.v s)))})
@@ -111,3 +113,6 @@ inline_for_extraction val mul_wide: a:limb -> b:limb -> Tot (c:wide{w c = v a * 
 
 inline_for_extraction val limb_to_wide: x:limb -> Tot (y:wide{w y = v x})
 inline_for_extraction val wide_to_limb: x:wide -> Tot (y:limb{v y = w x % pow2 limb_n})
+
+inline_for_extraction val uint64_to_limb: x:FStar.UInt64.t{FStar.UInt64.v x < pow2 word_size} ->
+  Tot (y:limb{v y = FStar.UInt64.v x})
