crypto/bignum/Hacl.Bignum.Fdifference.Spec.fst
@@ -1,0 +1,27 @@
+module Hacl.Bignum.Fdifference.Spec
+
+open Hacl.Bignum.Parameters
+open Hacl.Bignum.Bigint
+open Hacl.Bignum.Limb
+
+module U32 = FStar.UInt32
+
+#set-options "--initial_fuel 1 --max_fuel 1 --z3timeout 20"
+
+let gte_limbs (a:seqelem) (b:seqelem) (l:nat{l <= len}) : GTot Type0 =
+  (forall (i:nat). {:pattern (Seq.index a i) \/ (Seq.index b i)} i < l ==> v (Seq.index b i) >= v (Seq.index a i))
+
+
+val fdifference_spec:
+  a:seqelem -> b:seqelem ->
+  ctr:nat{ctr <= len /\ gte_limbs a b ctr} ->
+  Tot seqelem (decreases ctr)
+let rec fdifference_spec a b ctr =
+  if ctr = 0 then a
+  else (
+    let i = ctr - 1 in
+    let ai = Seq.index a i in
+    let bi = Seq.index b i in
+    let a' = Seq.upd a i (bi -^ ai) in
+    fdifference_spec a' b i
+  )
