crypto/bignum/Hacl.Bignum.Fproduct.Spec.fst
@@ -1,0 +1,217 @@
+module Hacl.Bignum.Fproduct.Spec
+
+open Hacl.Bignum.Parameters
+open Hacl.Bignum.Bigint
+open Hacl.Bignum.Limb
+open Hacl.Bignum.Modulo
+
+module U32 = FStar.UInt32
+
+#set-options "--initial_fuel 1 --max_fuel 1"
+
+let copy_from_wide_pre (s:seqelem_wide) : GTot Type0 =
+  (forall (i:nat). {:pattern w (Seq.index s i)} i < len ==> w (Seq.index s i) < pow2 n)
+
+
+#set-options "--z3timeout 20"
+
+val copy_from_wide_spec_: s:seqelem_wide{copy_from_wide_pre s} ->
+  i:nat{i <= len} ->
+  tmp:seqelem{(forall (j:nat). (j >= i /\ j < len) ==> v (Seq.index tmp j) = w (Seq.index s j))} ->
+  Tot (s':seqelem{(forall (j:nat). j < len ==> v (Seq.index s' j) = w (Seq.index s j))})
+let rec copy_from_wide_spec_ s i tmp =
+  if i = 0 then tmp
+  else (
+    let i = i - 1 in
+    let si = Seq.index s i in
+    let tmpi = wide_to_limb si in
+    Math.Lemmas.modulo_lemma (w si) (pow2 n);
+    let tmp' = Seq.upd tmp i tmpi in
+    copy_from_wide_spec_ s i tmp'
+  )
+
+
+#set-options "--z3timeout 5"
+
+val copy_from_wide_spec: s:seqelem_wide{copy_from_wide_pre s} ->
+  Tot (s':seqelem{(forall (j:nat). j < len ==> v (Seq.index s' j) = w (Seq.index s j))})
+let rec copy_from_wide_spec s =
+  let tmp = Seq.create len limb_zero in
+  copy_from_wide_spec_ s len tmp
+
+
+#set-options "--z3timeout 5"
+
+val shift_spec: seqelem -> Tot seqelem
+let shift_spec s =
+  let sfirst = Seq.slice s 0 (len - 1) in
+  let slast = Seq.slice s (len-1) len in
+  Seq.append slast sfirst
+
+#set-options "--z3timeout 20 --initial_fuel 1 --max_fuel 1"
+
+open FStar.Mul
+
+let sum_scalar_multiplication_pre_ (sw:seqelem_wide) (s:seqelem) (scalar:limb) (i:nat{i <= len}) : GTot Type0 =
+  (forall (j:nat). j < i ==> w (Seq.index sw j) + (v (Seq.index s j) * v scalar) < pow2 wide_n)
+
+
+val sum_scalar_multiplication_spec:
+  sw:seqelem_wide ->
+  s:seqelem ->
+  scalar:limb ->
+  i:nat{i <= len /\ sum_scalar_multiplication_pre_ sw s scalar i} ->
+  Tot seqelem_wide
+  (decreases i)
+let rec sum_scalar_multiplication_spec sw s scalar i =
+  if i = 0 then sw
+  else (
+    let j = i - 1 in
+    let swi = Seq.index sw j in
+    let si = Seq.index s j in
+    let open Hacl.Bignum.Wide in
+    let swi' = swi +^ (mul_wide si scalar) in
+    let sw' = Seq.upd sw j swi' in
+    sum_scalar_multiplication_spec sw' s scalar j
+  )
+
+
+let shift_reduce_pre (s:seqelem) : GTot Type0 = reduce_pre (shift_spec s)
+
+val shift_reduce_spec: s:seqelem{shift_reduce_pre s} -> Tot (s':seqelem)
+let shift_reduce_spec s =
+  reduce_spec (shift_spec s)
+
+
+let rec mul_shift_reduce_pre (output:seqelem_wide) (input:seqelem) (input2:seqelem) (ctr:nat{ctr <= len}) : GTot Type0 (decreases ctr) =
+  if ctr > 0 then (
+    sum_scalar_multiplication_pre_ output input (Seq.index input2 (len-ctr)) len
+    /\ (let output' = sum_scalar_multiplication_spec output input (Seq.index input2 (len-ctr)) len in
+       (ctr > 1 ==> shift_reduce_pre input) /\
+         (let input'  = if ctr > 1 then shift_reduce_spec input else input in
+          mul_shift_reduce_pre output' input' input2 (ctr-1))))
+          else true
+
+
+val mul_shift_reduce_spec:
+  output:seqelem_wide ->
+  input:seqelem -> input2:seqelem ->
+  ctr:nat{ctr <= len /\ mul_shift_reduce_pre output input input2 ctr} ->
+  Tot seqelem_wide
+  (decreases ctr)
+let rec mul_shift_reduce_spec output input input2 ctr =
+  if ctr = 0 then output
+  else (
+    let i = ctr - 1 in
+    let j = len - i - 1 in
+    let input2j = Seq.index input2 j in
+    let output' = sum_scalar_multiplication_spec output input input2j len in
+    let input'  = if ctr > 1 then shift_reduce_spec input else input in
+    mul_shift_reduce_spec output' input' input2 i
+  )
+
+
+#set-options "--z3timeout 10"
+
+let carry_wide_pre (s:seqelem_wide) (i:nat{i < len}) : GTot Type0 =
+  (forall (j:nat). {:pattern (w (Seq.index s j))} (j > i /\ j < len) ==> w (Seq.index s j) < pow2 (wide_n - 1))
+  /\ (forall (j:nat). {:pattern (w (Seq.index s j))} (j < i) ==> w (Seq.index s j) < pow2 limb_size)
+
+
+#set-options "--z3timeout 100 --initial_fuel 1 --max_fuel 1"
+
+val carry_wide_spec: s:seqelem_wide -> i:nat{i < len /\ carry_wide_pre s i} -> Tot (s':seqelem_wide)
+  (decreases (len - 1 - i))
+let rec carry_wide_spec s i =
+  if i = len - 1 then s
+  else (
+    let si = Seq.index s i in
+    let sip1 = Seq.index s (i+1) in
+    cut (w sip1 < pow2 (wide_n - 1));
+    assert_norm(pow2 0 = 1);
+    Math.Lemmas.pow2_lt_compat limb_size 0;
+    Math.Lemmas.pow2_lt_compat limb_n limb_size;
+    Math.Lemmas.modulo_lemma (pow2 limb_size) (pow2 limb_n);
+    let mask = (limb_one <<^ climb_size) -^ limb_one in
+    UInt.logand_mask #limb_n (v (wide_to_limb si)) limb_size;
+    let r0 = wide_to_limb si &^ mask in
+    Math.Lemmas.pow2_plus (limb_n - limb_size) (limb_size);
+    Math.Lemmas.modulo_modulo_lemma (w si) (pow2 limb_size) (pow2 (limb_n - limb_size));
+    assert(v r0 = w si % pow2 limb_size);
+    assert(v r0 < pow2 limb_size);
+    let open Hacl.Bignum.Wide in
+    let c = si >>^ climb_size in
+    Math.Lemmas.pow2_lt_compat (wide_n - 1) (limb_n);
+    Math.Lemmas.pow2_double_sum (wide_n - 1);
+    Math.Lemmas.lemma_div_lt (w si) (wide_n) (limb_size);
+    Math.Lemmas.pow2_le_compat (wide_n - 1) (wide_n - limb_size);
+    cut (w c < pow2 (wide_n - 1));
+    let s' = Seq.upd s i (limb_to_wide r0) in
+    assert(forall (j:nat). {:pattern (Seq.index s' j)} j < i + 1 ==> w (Seq.index s' j) < pow2 limb_size);
+    assert(forall (j:nat). {:pattern (Seq.index s' j)} (j > i /\ j < len) ==> w (Seq.index s' j) < pow2 (wide_n - 1));
+    let s'' = Seq.upd s' (i+1) (sip1 +^ c) in
+    assert(forall (j:nat). {:pattern (Seq.index s'' j)} j < i + 1 ==> w (Seq.index s'' j) < pow2 limb_size);
+    assert(forall (j:nat). {:pattern (Seq.index s'' j)} (j > i + 1 /\ j < len) ==> w (Seq.index s'' j) < pow2 (wide_n - 1));
+    carry_wide_spec s'' (i+1)
+  )
+
+
+#set-options "--z3timeout 5"
+
+
+let carry_0_to_1_pre (input:seqelem) : GTot Type0 =
+  (forall (i:nat). (i > 0 /\ i < len) ==> v (Seq.index input i) < pow2 limb_size)
+
+
+val carry_0_to_1_spec: input:seqelem{carry_0_to_1_pre input} -> Tot (output:seqelem)
+let carry_0_to_1_spec input =
+  assume (Seq.length input > 1);
+  let i0 = Seq.index input 0 in
+  let i1 = Seq.index input 1 in
+  assert_norm(pow2 0 = 1);
+  Math.Lemmas.pow2_lt_compat limb_size 0;
+  Math.Lemmas.pow2_lt_compat limb_n limb_size;
+  Math.Lemmas.modulo_lemma (pow2 limb_size) (pow2 limb_n);
+  let i0' = i0 &^ ((limb_one <<^ climb_size) -^ limb_one) in
+  UInt.logand_mask #limb_n (v i0) limb_size;
+  Math.Lemmas.pow2_plus (limb_n - limb_size) (limb_size);
+  Math.Lemmas.modulo_modulo_lemma (v i0) (pow2 limb_size) (pow2 (limb_n - limb_size));
+  let c = i0 >>^ climb_size in
+  Math.Lemmas.pow2_double_sum (limb_n - 1);
+  Math.Lemmas.pow2_le_compat (limb_n - 1) limb_size;
+  Math.Lemmas.lemma_div_lt (v i0) (limb_n) (limb_size);
+  Math.Lemmas.pow2_le_compat (limb_n - 1) (limb_n - limb_size);
+  let i1' = i1 +^ c in
+  let output = Seq.upd input 0 i0' in
+  Seq.upd output 1 i1'
+
+#set-options "--z3timeout 5"
+
+let fmul_pre (input:seqelem) (input2:seqelem) : GTot Type0 =
+  mul_shift_reduce_pre (Seq.create len wide_zero) input input2 len
+
+assume val lemma_mul_to_red: input:seqelem -> input2:seqelem -> Lemma
+  (requires (fmul_pre input input2))
+  (ensures  (fmul_pre input input2
+    /\ carry_wide_pre (mul_shift_reduce_spec (Seq.create len wide_zero) input input2 len) 0
+    /\ reduce_wide_pre (carry_wide_spec (mul_shift_reduce_spec (Seq.create len wide_zero) input input2 len) 0)
+    /\ copy_from_wide_pre (reduce_wide_spec (carry_wide_spec (mul_shift_reduce_spec (Seq.create len wide_zero) input input2 len) 0))
+    /\ carry_0_to_1_pre (copy_from_wide_spec (reduce_wide_spec (carry_wide_spec (mul_shift_reduce_spec (Seq.create len wide_zero) input input2 len) 0)))))
+
+
+val fmul_spec: input:seqelem -> input2:seqelem{fmul_pre input input2} -> Tot (output:seqelem)
+let fmul_spec input input2 =
+  lemma_mul_to_red input input2;
+  let tmp = Seq.create len wide_zero in
+  let output1 = mul_shift_reduce_spec tmp input input2 len in
+  let output2 = carry_wide_spec output1 0 in
+  let output3 = reduce_wide_spec output2 in
+  let output4 = copy_from_wide_spec output3 in
+  carry_0_to_1_spec output4
+
+#set-options "--z3timeout 40"
+
+
+val lemma_whole_slice: #a:Type -> s:Seq.seq a -> Lemma
+  (Seq.slice s 0 (Seq.length s) == s)
+let lemma_whole_slice #a s = Seq.lemma_eq_intro (Seq.slice s 0 (Seq.length s)) s
