crypto/bignum/Hacl.Bignum.Fscalar.Spec.fst
@@ -1,0 +1,20 @@
+module Hacl.Bignum.Fscalar.Spec
+
+open Hacl.Bignum.Parameters
+open Hacl.Bignum.Bigint
+open Hacl.Bignum.Limb
+
+module U32 = FStar.UInt32
+
+#set-options "--initial_fuel 1 --max_fuel 1 --z3timeout 20"
+
+val fscalar_spec: output:seqelem_wide -> input:seqelem -> s:limb -> ctr:nat{ctr <= len} -> Tot seqelem_wide (decreases ctr)
+let rec fscalar_spec output input s ctr =
+  if ctr = 0 then output
+  else (
+    let i = ctr - 1 in
+    let inputi = Seq.index input i in
+    let open Hacl.Bignum.Wide in
+    let output' = Seq.upd output i (inputi *^ s) in
+    fscalar_spec output' input s i
+  )
