crypto/bignum/Hacl.Bignum.Fsum.Spec.fst
@@ -1,0 +1,28 @@
+module Hacl.Bignum.Fsum.Spec
+
+open Hacl.Bignum.Parameters
+open Hacl.Bignum.Bigint
+open Hacl.Bignum.Limb
+open Hacl.Bignum.Predicates
+
+
+module U32 = FStar.UInt32
+
+#set-options "--max_fuel 1 --initial_fuel 1"
+
+let red (s:seqelem) (l:nat{l <= len}) = (forall (i:nat). (i < l) ==> v (Seq.index s i) < pow2 (n - 1))
+
+
+val fsum_spec: s:seqelem -> s':seqelem -> ctr:nat{ctr <= len /\ red s ctr /\ red s' ctr} -> Tot seqelem
+  (decreases ctr)
+let rec fsum_spec a b ctr =
+  if ctr = 0 then a
+  else (
+    let i = ctr - 1 in
+    let ai = Seq.index a i in
+    let bi = Seq.index b i in
+    Math.Lemmas.pow2_double_sum (n-1);
+    let a' = Seq.upd a i (ai +^ bi) in
+    fsum_spec a' b i
+  )
+
