crypto/bignum/x25519/Blah.fst
@@ -1,0 +1,5 @@
+module Blah
+
+open Test
+
+let test () = assert(x = 3)
