crypto/bignum/x25519/Hacl.Bignum.Constants.fst
@@ -1,0 +1,6 @@
+module Hacl.Bignum.Constants
+
+inline_for_extraction let prime = assert_norm(pow2 255 > 19); pow2 255 - 19
+inline_for_extraction let word_size = 64
+inline_for_extraction let len = 5
+inline_for_extraction let limb_size = 51
