crypto/bignum/x25519/Hacl.Bignum.Crecip.fst
@@ -1,0 +1,42 @@
+module Hacl.Bignum.Crecip
+
+open FStar.HyperStack
+open FStar.Buffer
+
+open Hacl.Bignum.Parameters
+open Hacl.Bignum.Bigint
+open Hacl.Bignum.Limb
+open Hacl.Bignum.Fproduct
+
+module U32 = FStar.UInt32
+
+let crecip out z =
+  push_frame();
+  let buf = create zero_64 20ul in
+  let a  = Buffer.sub buf 0ul  5ul in
+  let t0 = Buffer.sub buf 5ul  5ul in
+  let b  = Buffer.sub buf 10ul 5ul in
+  let c  = Buffer.sub buf 15ul 5ul in
+  fsquare_times a z 1ul;
+  fsquare_times t0 a 2ul;
+  fmul b t0 z;
+  fmul a b a;
+  fsquare_times t0 a 1ul;
+  fmul b t0 b;
+  fsquare_times t0 b 5ul;
+  fmul b t0 b;
+  fsquare_times t0 b 10ul;
+  fmul c t0 b;
+  fsquare_times t0 c 20ul;
+  fmul t0 t0 c;
+  fsquare_times t0 t0 10ul;
+  fmul b t0 b;
+  fsquare_times t0 b 50ul;
+  fmul c t0 b;
+  fsquare_times t0 c 100ul;
+  fmul t0 t0 c;
+  fsquare_times t0 t0 50ul;
+  fmul t0 t0 b;
+  fsquare_times t0 t0 5ul;
+  fmul out t0 a;
+  pop_frame()
