crypto/bignum/x25519/Hacl.Bignum.Modulo.fst
@@ -1,0 +1,105 @@
+module Hacl.Bignum.Modulo
+
+open FStar.Mul
+open FStar.HyperStack
+open FStar.Buffer
+
+open Hacl.Bignum.Parameters
+open Hacl.Bignum.Bigint
+open Hacl.Bignum.Limb
+
+#set-options "--lax"
+
+inline_for_extraction let two54m152 = uint64_to_limb 0x3fffffffffff68uL
+inline_for_extraction let two54m8   = uint64_to_limb 0x3ffffffffffff8uL
+inline_for_extraction let nineteen  = uint64_to_limb 19uL
+inline_for_extraction let mask_51    = uint64_to_limb 0x7ffffffffffffuL
+
+let add_zero_pre s =
+  let _ = () in
+  v (Seq.index s 0) < pow2 63
+  /\ v (Seq.index s 1) < pow2 63
+  /\ v (Seq.index s 2) < pow2 63
+  /\ v (Seq.index s 3) < pow2 63
+  /\ v (Seq.index s 4) < pow2 63
+
+
+let add_zero_spec s =
+  let s = Seq.upd s 0 (Seq.index s 0 +^ two54m152) in
+  let s = Seq.upd s 1 (Seq.index s 1 +^ two54m8) in
+  let s = Seq.upd s 2 (Seq.index s 2 +^ two54m8) in
+  let s = Seq.upd s 3 (Seq.index s 3 +^ two54m8) in
+  Seq.upd s 4 (Seq.index s 4 +^ two54m8)
+
+
+let add_zero b =
+  let b0 = b.(0ul) in
+  let b1 = b.(1ul) in
+  let b2 = b.(2ul) in
+  let b3 = b.(3ul) in
+  let b4 = b.(4ul) in
+  b.(0ul) <- b0 +^ two54m152;
+  b.(1ul) <- b1 +^ two54m8;
+  b.(2ul) <- b2 +^ two54m8;
+  b.(3ul) <- b3 +^ two54m8;
+  b.(4ul) <- b4 +^ two54m8
+
+let carry_top_pre s =
+  let _ = () in
+  19 * v (Seq.index s 4) + v (Seq.index s 0) < pow2 64
+
+let carry_top_spec s =
+  let s4 = Seq.index s 4 in
+  let s0 = Seq.index s 0 in
+  let mask = (limb_one <<^ climb_size) -^ limb_one in
+  let nineteen = (limb_one <<^ 4ul) +^ (limb_one <<^ 1ul) +^ limb_one in
+  let s4' = s4 &^ mask in
+  let s0' = s0 +^ (nineteen *^ (s4 >>^ climb_size)) in
+  let s = Seq.upd s 4 s4' in
+  Seq.upd s 0 s0'
+
+let carry_top b =
+  let b4 = b.(4ul) in
+  let b0 = b.(0ul) in
+  let mask = (limb_one <<^ climb_size) -^ limb_one in
+  let nineteen = (limb_one <<^ 4ul) +^ (limb_one <<^ 1ul) +^ limb_one in
+  let b4' = b4 &^ mask in
+  let b0' = b0 +^ (nineteen *^ (b4 >>^ climb_size)) in
+  b.(4ul) <- b4';
+  b.(0ul) <- b0'
+
+
+let reduce_pre s =
+  let _ = () in
+  v (Seq.index s 0) * 19 < pow2 64
+
+
+let reduce_spec s =
+  let nineteen = (limb_one <<^ 4ul) +^ (limb_one <<^ 1ul) +^ limb_one in
+  let s0 = Seq.index s 0 in
+  Seq.upd s 0 (s0 *^ nineteen)
+
+
+let reduce b =
+  let nineteen = (limb_one <<^ 4ul) +^ (limb_one <<^ 1ul) +^ limb_one in
+  let b0 = b.(0ul) in
+  b.(0ul) <- nineteen *^ b0
+
+
+let reduce_wide_pre s =
+  let _ = () in
+  w (Seq.index s 0) * 19 < pow2 128
+
+
+let reduce_wide_spec s =
+  let open Hacl.Bignum.Wide in
+  let s0 = Seq.index s 0 in
+  let s0_19 = (s0 <<^ 4ul) +^ (s0 <<^ 1ul) +^ s0 in
+  Seq.upd s 0 (s0_19)
+
+
+let reduce_wide b =
+  let s0 = b.(0ul) in
+  let open Hacl.Bignum.Wide in
+  let s0_19 = (s0 <<^ 4ul) +^ (s0 <<^ 1ul) +^ s0 in
+  b.(0ul) <- s0_19
