crypto/bignum/x25519/Hacl.EC.AddAndDouble.fst
@@ -1,0 +1,47 @@
+module Hacl.EC.AddAndDouble
+
+open FStar.HyperStack
+open FStar.Buffer
+
+
+let fmonty x2 z2 x3 z3 x z xprime zprime qmqp =
+  let x2 = getx pp in
+  let z2 = getz pp in
+  let x3 = getx ppq in
+  let z3 = getz ppq in
+  let x  = getx p in
+  let z  = getz p in
+  let xprime  = getx pq in
+  let zprime  = getz pq in
+  push_frame();
+  let buf = create zero_64 40ul in
+  let origx      = Buffer.sub buf 0ul  5ul in
+  let origxprime = Buffer.sub buf 5ul  5ul in
+  let zzz        = Buffer.sub buf 10ul 5ul in
+  let xx         = Buffer.sub buf 15ul 5ul in
+  let zz         = Buffer.sub buf 20ul 5ul in
+  let xxprime    = Buffer.sub buf 25ul 5ul in
+  let zzprime    = Buffer.sub buf 30ul 5ul in
+  let zzzprime   = Buffer.sub buf 35ul 5ul in
+  blit x 0ul origx 0ul 5ul;
+  fsum x z; // x < x + z
+  fdifference z origx; // z <- 8p + x - z
+  blit xprime 0ul origxprime 0ul 5ul;
+  fsum xprime zprime; // xprime <- xprime + zprime
+  fdifference zprime origxprime; // zprime <- 8p + xprime - zprime
+  fmul xxprime xprime z; // xxprime <- sum * sub
+  fmul zzprime x zprime; // zzprime <- sum * sub
+  blit xxprime 0ul origxprime 0ul 5ul;
+  fsum xxprime zzprime; // xxprime <- sum
+  fdifference zzprime origxprime; // zzprime <- sub
+  fsquare_times x3 xxprime 1ul; // sum sum
+  fsquare_times zzzprime zzprime 1ul; // sub sub 
+  fmul z3 zzzprime qmqp;
+  fsquare_times xx x 1ul; // sum red
+  fsquare_times zz z 1ul; // red sub 
+  fmul x2 xx zz; // red red
+  fdifference zz xx; // red red
+  fscalar_product zzz zz (uint64_to_sint64 121665uL);
+  fsum zzz xx; // red red
+  fmul z2 zz zzz;
+  pop_frame()
