crypto/bignum/x25519/Hacl.EC.Point.fst
@@ -1,0 +1,27 @@
+module Hacl.EC.Point
+
+open FStar.Mul
+open FStar.HyperStack
+open FStar.Ghost
+open FStar.Buffer
+
+open Hacl.Bignum.Parameters
+open Hacl.Bignum.Bigint
+open Hacl.Bignum.Limb
+open Hacl.Bignum
+
+module U32 = FStar.UInt32
+
+let plen = 10
+let cplen = 10ul
+
+let getx p = Buffer.sub p 0ul 5ul
+let gety p = Buffer.sub p 0ul 5ul
+let getz p = Buffer.sub p 5ul 5ul
+
+let live_coords h x y z = live h x /\ live h z
+
+let live h p = live_coords h (getx p) (gety p) (getz p)
+
+let make x y z = admit()
+
